Cslib/Computability/Machines/MultiTapeTuring/Routines/Navigation.lean
@@ -13,56 +13,79 @@ public import Cslib.Computability.Machines.MultiTapeTuring.Routines.Skip
 namespace Turing
 namespace Routines
 
--- ═══════════════════════════════════════════════════════════════════════════
--- Argument navigation (for Data.list values)
--- ═══════════════════════════════════════════════════════════════════════════
+
+public def onNonemptyList {k : ℕ} (i : Fin k) (tm : MultiTapeTM k Char) :
+    MultiTapeTM k Char :=
+  if_eq '(' i
+    (right i ;ₜ if_eq '(' i (left i ;ₜ tm) (left i ;ₜ left i))
+    (noop)
+
+/-- Execute `tm` if the current element is a non-empty list. Otherwise, do nothing. -/
+@[simp]
+public lemma onNonemptylist.eval_struct {k : ℕ} {i : Fin k} (tm : MultiTapeTM k Char)
+    {views : Fin k → TapeView} :
+  (onNonemptyList i tm).eval_struct views =
+    if (views i).currentList.isSome then tm.eval_struct views else Part.some views := by
+  simp [onNonemptyList]
+  sorry
+
+@[simp]
+public lemma right_on_nonempty_list {k : ℕ} {i : Fin k}
+    {views : Fin k → TapeView}
+    {ls : List Data}
+    (h_list : (views i).current = some (Data.list ls))
+    (h_nonempty : 0 < ls.length) :
+    (right i).eval_struct views = some
+      (Function.update views i (((views i).toElem? 0).get (by simp [h_list, h_nonempty]))) := by
+  sorry
 
 def skipRight_n {k : ℕ} (n : ℕ) (i : Fin k) : MultiTapeTM k Char :=
   match n with
   | 0 => noop
   | n + 1 => skipRight_n n i ;ₜ skipRight i
 
-@[simp]
-lemma skipRight_n.eval_struct {k : ℕ} {n : ℕ} {i : Fin k} {views : Fin k → TapeView}
-    (path : List ℕ)
-    (h_path : (views i).path = path ++ [idx])
-    (h_hasNextN : ((views i).data.atPath (path ++ [idx + n])).isSome) :
+lemma skipRight_n.eval_struct {j n : ℕ} {k : ℕ} {i : Fin k} {views : Fin k → TapeView}
+    {parent : TapeView}
+    {list : List Data}
+    (h_len : j + n < list.length)
+    (h_parent : parent.current = some (Data.list list))
+    (h_list : views i = ⟨parent.data, parent.path ++ [j]⟩) :
     (skipRight_n n i).eval_struct views = some
-      (Function.update views i
-        ⟨(views i).data, path ++ [idx + n]⟩) := by
-  induction n generalizing path with
-  | zero => simp [skipRight_n]; ext1 <;> simp [h_path]
+      (Function.update views i ⟨parent.data, parent.path ++ [j + n]⟩) := by
+  induction n with
+  | zero => simp [skipRight_n, h_list]
   | succ n ih =>
-    simp [skipRight_n]
-    let ih' := ih path h_path (by sorry)--simp [← Nat.add_assoc] at h_hasNextN; simp [h_hasNextN])
-    rw [ih']
-    simp
+     simp [skipRight_n, h_list]
+     rw [ih (by omega)]
+     simp
+     have h_next : (TapeView.mk parent.data (parent.path ++ [j + n])).next.isSome := by sorry
+     rw [skipRight_eval_struct (by grind)]
+     · simp [Nat.add_assoc]
+     · sorry
+     · sorry
 
-
-
-    sorry
 
 /-- Navigate to the `idx`-th element of a `Data.list` encoding on tape `i`.
 Moves past `(` and then skips `idx` Data elements.
 If `i` is larger than the length of the list, does nothing. -/
 public def toElem {k : ℕ} (idx : ℕ) (i : Fin k) : MultiTapeTM k Char :=
-  right i
-
-/-- If positioned on the element of a list, navigates to the list containing it. -/
-public def outOfList {k : ℕ} (i : Fin k) : MultiTapeTM k Char :=
-  left i ;ₜ while_eq ')' i (right i ;ₜ skipLeft i ;ₜ left i) ;ₜ
-    -- This part handles the case where we started out with a number on the tape or
-    -- an empty tape.
-    if_eq '(' i noop (right i)
+  right i ;ₜ skipRight_n idx i
 
 
 /-- `toElem idx i` moves to the `idx`th element of the `Data.list` currently pointed to
-on tape `i`. Only descends if the current element is a `Data.list` with at least `idx` elements,
-otherwise, the `TapeView` is unchanged. -/
+on tape `i`. -/
 @[simp]
-public lemma toElem_eval_struct {k : ℕ} {idx : ℕ} {i : Fin k} {views : Fin k → TapeView} :
+public lemma toElem_eval_struct {k : ℕ} {idx : ℕ} {i : Fin k} {views : Fin k → TapeView}
+  {list : List Data}
+  {h_isList : (views i).current = some (Data.list list)}
+  {h_len : idx < list.length} :
   (toElem idx i).eval_struct views = some
-    (Function.update views i (((views i).toElem? idx).getD (views i))) := by sorry
+    (Function.update views i ⟨(views i).data, (views i).path ++ [idx]⟩) := by
+  have h_nonempty : 0 < list.length := by omega
+  simp only [toElem, seq_eval_struct, h_isList, Option.some.injEq, Data.list.injEq, h_nonempty,
+    right_on_nonempty_list, TapeView.toElem?, Part.coe_some, Part.bind_some]
+  rw [skipRight_n.eval_struct (j := 0) (by simp [h_len]) h_isList (by simp)]
+  simp
 
 -- lemma outOfList_inner {k : ℕ} {i : Fin k} {views : Fin k → TapeView} :
 --   (right i ;ₜ skipLeft i ;ₜ left i).eval (toBiTape ∘ views) =
@@ -71,6 +94,14 @@ public lemma toElem_eval_struct {k : ℕ} {idx : ℕ} {i : Fin k} {views : Fin k
 --         if (views i).current = some (Data.list (_ :: _)) then
 --           some (Function.update views i ⟨(views i).data, (views i).path.dropLast⟩)
 --         else some views := by sorry
+
+/-- If positioned on the element of a list, navigates to the list containing it. -/
+public def outOfList {k : ℕ} (i : Fin k) : MultiTapeTM k Char :=
+  left i ;ₜ while_eq ')' i (right i ;ₜ skipLeft i ;ₜ left i) ;ₜ
+    -- This part handles the case where we started out with a number on the tape or
+    -- an empty tape.
+    if_eq '(' i noop (right i)
+
 
 /-- `outOfArg argIdx i` ascends back from the `argIdx`-th element,
     removing it from the end of the path. If the path ends with `argIdx`,
